Add traces to the concurrent semantics.
Traces are incorporated as part of a layer's state. When defining a layer, one
specifies a projection State -> list Event.

Very little is assumed about this function, other than that crash steps
preserve the trace. However, one probably wants to show that the top/bottom
layers of the stack have the property that this list is monotonically growing
as steps are taken.

The correctness criteria for layer refinement now require that
if we start executing from a state where the abstraction relation holds, then
after each step of execution of the concrete program, there exists a partial
execution of the abstract program which has an identical trace (we may want to
change this to be a *prefix* rather than equality). This trace property
continues to hold after crashes throughout recovery.

This property is a little odd unless the traces monotonically grow because the
partial execution of the abstract program that we match with after each step
need not be the same.

src/Spec/Abstraction.v
@@ -16,6 +16,12 @@ Section Abstraction.
              (spec: relation AState AState T) :=
     (absr;; p) ---> (v <- spec; absr;; pure v).
 
+  Definition refines_if T
+             (r: relation AState CState unit)
+             (p: relation CState CState T)
+             (spec: relation AState AState T) :=
+    (absr;; p) ---> (v <- spec; r;; pure v).
+
   Theorem refine_unfolded_iff T
           (p: relation CState CState T)
           (spec: relation AState AState T) :
@@ -45,6 +51,25 @@ Section Abstraction.
     refines p spec.
   Proof. eapply refine_unfolded_iff. Qed.
 
+  Theorem refine_if_unfolded_iff T r
+          (p: relation CState CState T)
+          (spec: relation AState AState T) :
+    (forall s s__a, absr s__a s tt ->
+             forall s' v, p s s' v ->
+                     exists s__a', spec s__a s__a' v /\
+                            r s__a' s' tt) <->
+    refines_if r p spec.
+  Proof.
+    unfold refines_if, rimpl, and_then, pure; split.
+    - propositional.
+      destruct o1.
+      eapply H in H0; eauto; propositional.
+      eauto 10.
+    - intros. edestruct H; eauto. propositional.
+      destruct o1.
+      eauto 10.
+  Qed.
+
   (* define refinement as transforming an abstract specification to a concrete
   one (a program satisfying the abstract spec should satisfy the concrete spec
   after refinement-preserving compilation) *)
@@ -70,6 +95,8 @@ Section Abstraction.
     Notation c_rec_seq := (rec_seq C_Op).
     Notation c_exec := c_sem.(exec).
     Notation c_rexec := c_sem.(rexec).
+    Notation c_exec_halt := c_sem.(exec_halt).
+    Notation c_rexec_partial := c_sem.(rexec_partial).
 
     Definition crash_refines T
                (p: c_proc T) (rec: c_rec_seq)
@@ -77,6 +104,13 @@ Section Abstraction.
                (rexec_spec: relation AState AState _) :=
       refines (c_exec p) exec_spec /\
       refines (c_rexec p rec) rexec_spec.
+
+    Definition halt_refines T r
+               (p: c_proc T) (rec: c_rec_seq)
+               (exec_partial_spec: relation AState AState _)
+               (rexec_partial_spec: relation AState AState _) :=
+      refines_if r (c_exec_halt p) exec_partial_spec /\
+      refines_if r (c_rexec_partial p rec) rexec_partial_spec.
   End Dynamics.
 
 End Abstraction.
